Fix more adequacy

src/heaplang/adequacy.v
@@ -1,97 +1,9 @@
 From ITree Require Import ITree Recursion RecursionFacts InterpFacts TranslateFacts Eqit.
 From iris Require Import invariants ghost_map.
 From iris.proofmode Require Import proofmode.
-From iris.program_logic Require Import language.
-From iris.itree Require Import wpi ub itree choice state later handler.
+From iris.itree Require Import wpi ub itree choice state later handler void.
 From iris.itree.threadpool Require Import ctrace handler interleaving.
 From iris.itree.heaplang Require Import lang.
-
-Inductive voidE : Type → Type :=.
-
-Section handler.
-  Context {Σ : gFunctors}.
-
-  Program Definition voidH : iHandler Σ voidE :=
-    IHandler (λ A e, match e with end )%I _.
-  Next Obligation. by move => ? []. Qed.
-  Global Instance voidH_Sequential :
-    Sequential voidH.
-  Proof. by iIntros (A [] Φ s) "HH". Qed.
-End handler.
-
-Definition insert_voidE {E R} (t : itree E R) : itree (E +' voidE) R :=
-  translate inl1 t.
-
-Lemma normalize_itree_translate_Ret {E F R} h (x : R) :
-  NormalizeITree true (translate (E:=E) (F:=F) h (Ret x)) (Ret x).
-Proof. constructor. by rewrite translate_ret. Qed.
-Global Hint Resolve normalize_itree_translate_Ret : itree_auto.
-
-Lemma normalize_itree_translate_Tau {E F R} h (t : itree E R) t' p :
-  NormalizeITree p (translate h t) t' →
-  NormalizeITree true (translate (E:=E) (F:=F) h (Tau t)) t'.
-Proof. move => [Heq]. constructor. by rewrite -Heq translate_tau tau_eutt. Qed.
-Global Hint Resolve normalize_itree_translate_Tau : itree_auto.
-
-Lemma normalize_itree_translate_Vis {E F R} A e h (k : A →itree E R) t' p :
-  NormalizeITree p (Vis (h _ e) (λ x, translate h (k x))) t' →
-  NormalizeITree true (translate (E:=E) (F:=F) h (Vis e k)) t'.
-Proof. move => [Heq]. constructor. by rewrite -Heq translate_vis. Qed.
-Global Hint Resolve normalize_itree_translate_Vis : itree_auto.
-
-
-Section adequacy.
-  Context {R : Type} {E : Type → Type}.
-  Context `{!invGS_gen hlc Σ} {H : iHandler Σ E}.
-
-  Theorem voidE_adequacy_empty (t : itree E R) Φ :
-    WPi t @ H; ∅ {{ Φ }} -∗
-    WPi insert_voidE t @ H ⊕ voidH; ∅ {{ Φ }}.
-  Proof.
-    iRevert (t Φ). rewrite /insert_voidE. iApply wpi_iter'; first solve_proper.
-    - iIntros "!>" (Φ t) "Hwp". wpi_norm. by iApply wpi_ret'.
-    - iIntros "!>" (Φ t) "Hwp". wpi_norm. by iApply wpi_update.
-    - iIntros "!>" (Φ A e k) "HH". wpi_norm.
-      iApply wpi_vis => /=. iMod "HH". iModIntro.
-      iApply ihandler_mono; last done.
-      + iIntros (a) "Hwp". by iApply wpi_update_post.
-      + iIntros "!>" (a) "Hwp". iApply wpi_clear_mask.
-        iMod "Hwp". iModIntro. iApply wpi_wand; last done.
-        iIntros (r []).
-  Qed.
-
-  Theorem voidE_adequacy (t : itree E R) Φ M :
-    WPi t @ H; M {{ Φ }} -∗
-    WPi insert_voidE t @ H ⊕ voidH; M {{ Φ }}.
-  Proof.
-    iIntros "Hwp".
-    rewrite -wpi_clear_mask. iEval (rewrite -wpi_clear_mask).
-    iMod "Hwp". iModIntro.
-    iPoseProof voidE_adequacy_empty as "Had". iSpecialize ("Had" with "Hwp").
-    iApply wpi_wand; last done. iIntros (r). eauto.
-  Qed.
-
-  Theorem voidE_terminates_empty_mask (t : itree voidE R) Φ :
-    WPi t @ voidH; ∅ {{ Φ }} -∗
-    |={∅}=> ∃ v, ⌜t ≈ Ret v⌝ ∗ Φ v.
-  Proof.
-    iRevert (t Φ). iApply wpi_iter'; first solve_proper.
-    - iIntros "!>" (Φ t) ">$". by iModIntro.
-    - iIntros "!>" (Φ t) ">>[% [% $]]". iModIntro. by rewrite tau_eutt.
-    - iIntros "!>" (Φ A [] k) "HH".
-  Qed.
-
-  Theorem voidE_terminates (t : itree voidE R) Φ M :
-    WPi t @ voidH; M {{ Φ }} -∗
-    |={M, ∅}=> ∃ v, ⌜t ≈ Ret v⌝ ∗ |={∅,M}=> Φ v.
-  Proof.
-    iIntros "Hwp".
-    rewrite -wpi_clear_mask. iMod "Hwp".
-    iMod (voidE_terminates_empty_mask with "Hwp") as (? ?) "$".
-    done.
-  Qed.
-End adequacy.
-
 
 Definition heaplang_irel {R} (t : itree heaplangE R) (σ : state) (n : option nat)
   (te : itree voidE (option ((state * (R + last_thread_killed)) + later_exhausted))) : Prop :=
@@ -151,5 +63,6 @@ Section adequacy.
     iIntros (? ?) "Hs Hlc Hwp".
     iApply (heaplang_adequacy_irel with "Hs Hlc"); [done..|].
     iApply wpi_bind. iApply wpi_wand; [|done]. iIntros (?) "?".
-  Admitted.
+    iApply wpi_bind. iApply wpi_yield_if_not_val. by iApply wpi_ret.
+  Qed.
 End adequacy.
