src/void.v
@@ -1,0 +1,72 @@
+From ITree Require Import ITree Eqit.
+From iris.proofmode Require Import proofmode.
+From iris.base_logic.lib Require Import iprop fancy_updates.
+From iris.itree Require Import wpi itree handler.
+
+Inductive voidE : Type → Type :=.
+
+Section handler.
+  Context {Σ : gFunctors}.
+
+  Program Definition voidH : iHandler Σ voidE :=
+    IHandler (λ A e, match e with end )%I _.
+  Next Obligation. by move => ? []. Qed.
+  Global Instance voidH_Sequential :
+    Sequential voidH.
+  Proof. by iIntros (A [] Φ s) "HH". Qed.
+End handler.
+
+Definition insert_voidE {E R} (t : itree E R) : itree (E +' voidE) R :=
+  translate inl1 t.
+
+Section adequacy.
+  Context {R : Type} {E : Type → Type}.
+  Context `{!invGS_gen hlc Σ} {H : iHandler Σ E}.
+
+  Theorem voidE_adequacy_empty (t : itree E R) Φ :
+    WPi t @ H; ∅ {{ Φ }} -∗
+    WPi insert_voidE t @ H ⊕ voidH; ∅ {{ Φ }}.
+  Proof.
+    iRevert (t Φ). rewrite /insert_voidE. iApply wpi_iter'; first solve_proper.
+    - iIntros "!>" (Φ t) "Hwp". wpi_norm. by iApply wpi_ret'.
+    - iIntros "!>" (Φ t) "Hwp". wpi_norm. by iApply wpi_update.
+    - iIntros "!>" (Φ A e k) "HH". wpi_norm.
+      iApply wpi_vis => /=. iMod "HH". iModIntro.
+      iApply ihandler_mono; last done.
+      + iIntros (a) "Hwp". by iApply wpi_update_post.
+      + iIntros "!>" (a) "Hwp". iApply wpi_clear_mask.
+        iMod "Hwp". iModIntro. iApply wpi_wand; last done.
+        iIntros (r []).
+  Qed.
+
+  Theorem voidE_adequacy (t : itree E R) Φ M :
+    WPi t @ H; M {{ Φ }} -∗
+    WPi insert_voidE t @ H ⊕ voidH; M {{ Φ }}.
+  Proof.
+    iIntros "Hwp".
+    rewrite -wpi_clear_mask. iEval (rewrite -wpi_clear_mask).
+    iMod "Hwp". iModIntro.
+    iPoseProof voidE_adequacy_empty as "Had". iSpecialize ("Had" with "Hwp").
+    iApply wpi_wand; last done. iIntros (r). eauto.
+  Qed.
+
+  Theorem voidE_terminates_empty_mask (t : itree voidE R) Φ :
+    WPi t @ voidH; ∅ {{ Φ }} -∗
+    |={∅}=> ∃ v, ⌜t ≈ Ret v⌝ ∗ Φ v.
+  Proof.
+    iRevert (t Φ). iApply wpi_iter'; first solve_proper.
+    - iIntros "!>" (Φ t) ">$". by iModIntro.
+    - iIntros "!>" (Φ t) ">>[% [% $]]". iModIntro. by rewrite tau_eutt.
+    - iIntros "!>" (Φ A [] k) "HH".
+  Qed.
+
+  Theorem voidE_terminates (t : itree voidE R) Φ M :
+    WPi t @ voidH; M {{ Φ }} -∗
+    |={M, ∅}=> ∃ v, ⌜t ≈ Ret v⌝ ∗ |={∅,M}=> Φ v.
+  Proof.
+    iIntros "Hwp".
+    rewrite -wpi_clear_mask. iMod "Hwp".
+    iMod (voidE_terminates_empty_mask with "Hwp") as (? ?) "$".
+    done.
+  Qed.
+End adequacy.
